Make all arguments to state monad implicit.

lib/Monads/State.v
@@ -3,20 +3,20 @@ Require Import Monads.Monad.
 Open Scope monad.
 
 
-Definition state_monad (State: Type) (Exception: Type) (Result: Type) :=
+Definition state_monad {State Exception Result: Type} :=
   State -> (Result + Exception) * State.
 
-Definition state_return (State Exception Result: Type) (res: Result) : state_monad State Exception Result :=
+Definition state_return {State Exception Result: Type} (res: Result) : @state_monad State Exception Result :=
   fun env => (inl res, env).
   
-Definition state_fail (State Exception Result: Type) (exc: Exception) : state_monad State Exception Result :=
+Definition state_fail {State Exception Result: Type} (exc: Exception) : @state_monad State Exception Result :=
   fun env => (inr exc, env).
 
 Definition state_bind
-  (State Exception Result Result': Type)
-  (c: state_monad State Exception Result)
-  (f: Result -> state_monad State Exception Result') 
-  : state_monad State Exception Result' :=
+  {State Exception Result Result': Type}
+  (c: @state_monad State Exception Result)
+  (f: Result -> @state_monad State Exception Result') 
+  : @state_monad State Exception Result' :=
   fun env =>
     let (ret, env') := c env in
     match ret with 
@@ -24,7 +24,7 @@ Definition state_bind
     | inr exc => (inr exc, env')
     end.
     
-Global Instance state_monad_inst (State Exception: Type) : Monad (state_monad State Exception) :=
-  { mret := state_return State Exception;
-    mbind := state_bind State Exception
+Global Instance state_monad_inst {State Exception: Type} : Monad (@state_monad State Exception) :=
+  { mret := @state_return State Exception;
+    mbind := @state_bind State Exception
   }.
